theories/BlockFusion.v
@@ -10,7 +10,14 @@ Import gmap Block Head.
 Import Map MapF MapF.P MapF.P.F.
 Import IdOT MapCFG Head Focus Block Patterns. *)
 
-Definition is_seq (A: blk) (id: bid) := if decide (successors A = {[id]}) then true else false.
+(*  Look at the terminator directly.
+    We would like to be able to use [successors],
+    but that would cause equivalence problems when the condition is a poison value.
+    *)
+Definition is_seq (A: blk) (id: bid) := match A.(blk_term) with
+  | TERM_Br_1 id' => if decide (id=id') then true else false
+  | _ => false
+end.
 
 Definition BlockFusion_f {S}: (bid * blk * (bid * blk * S) → bool) := fun '(_, A, (idB, _, _)) => is_seq A idB.
 
@@ -23,16 +30,16 @@ Record BlockFusion_sem idA A idB B (G G': ocfg): Prop := {
   INA: G !! idA = Some A;
   INB: G !! idB = Some B;
   PRED: predecessors idB G = {[idA]};
-  SUC: successors A = {[idB]}
+  SUC: A.(blk_term) = TERM_Br_1 idB
 }.
 
 Lemma is_seq_correct:
   forall A id, is_seq A id = true <->
-  successors A = {[id]}.
+  A.(blk_term) = TERM_Br_1 id.
 Proof.
   unfold is_seq. intros A id. split; intro SUC.
-  - now break_match_hyp.
-  - now break_match_goal.
+  - case_match; try discriminate. now case_match; subst.
+  - case_match; try discriminate. case_match; auto. inversion SUC. now subst.
 Qed.
 
 Lemma emptyunion: forall (m: gset bid), m = m∪∅.
@@ -58,14 +65,16 @@ Proof.
     * now simplify_map_eq.
     * assert (EQ: G = <[idA:=A]> G') by (subst G'; now rewrite insert_delete). rewrite EQ. rewrite predecessors_insert.
       rewrite PRED0. assert (EQp: predecessors_acc idB idA A = {[idA]}).
-      unfold predecessors_acc, is_predecessor. break_match_goal. trivial. break_match_hyp. discriminate. set_solver.
+      unfold predecessors_acc, is_predecessor. break_match_goal. trivial. break_match_hyp. discriminate.
+      unfold successors in n. rewrite SUCC in n. cbn in n. set_solver.
       rewrite EQp. set_solver. subst. now simplify_map_eq.
   - intros (G' & INX & [EQ NEQ INA INB PRED SUC]). split; trivial. exists (delete idA G). split. split; trivial.
     exists G'. split; trivial. split; trivial. now simplify_map_eq.
     pose proof insert_delete G _ _ INA as INDE. rewrite <- INDE in PRED.
     rewrite predecessors_insert in PRED. 
     assert (EQp: predecessors_acc idB idA A = {[idA]}). {
-      unfold predecessors_acc, is_predecessor. break_match_goal. trivial. break_match_hyp. discriminate. set_solver.
+      unfold predecessors_acc, is_predecessor. break_match_goal. trivial. break_match_hyp. discriminate.
+      unfold successors in n. rewrite SUC in n. cbn in n. set_solver.
     }
     pose proof emptyunion {[idA]} as Ee. rewrite Ee in PRED.
     rewrite EQp in PRED.
